TensorLib/Bytes.lean
@@ -5,68 +5,107 @@ Authors: Jean-Baptiste Tristan, Paul Govereau, Sean McLaughlin
 -/
 
 import TensorLib.Common
-
 namespace TensorLib
+
+class ToLEByteArray (a : Type) where
+  toLEByteArray : a -> ByteArray
+
+export ToLEByteArray(toLEByteArray)
+
+class ToBEByteArray (a : Type) where
+  toBEByteArray : a -> ByteArray
+
+export ToBEByteArray(toBEByteArray)
+
+instance : ToLEByteArray ByteArray where
+  toLEByteArray arr := arr
+
+instance : ToBEByteArray ByteArray where
+  toBEByteArray arr := arr
 
 -- We cast between UIntX and ByteArray without going through BitVec, which is represented
 -- as a Nat at runtime. We'll have tests for these in our ByteArray extension module where we
 -- have conversions back and forth between LE ByteArrays and UIntX.
-def _root_.UInt8.toLEByteArray (n : UInt8) : ByteArray := ByteArray.mk #[n]
-def _root_.UInt8.toBEByteArray (n : UInt8) : ByteArray := ByteArray.mk #[n]
+instance : ToLEByteArray UInt8 where
+  toLEByteArray n := ByteArray.mk #[n]
 
-def _root_.UInt16.toLEByteArray (n : UInt16) : ByteArray :=
-  let b0 := (n      ).toUInt8
-  let b1 := (n >>> 8).toUInt8
-  ByteArray.mk #[b0, b1]
+instance : ToBEByteArray UInt8 where
+  toBEByteArray n := ByteArray.mk #[n]
 
-def _root_.UInt16.toBEByteArray (n : UInt16) : ByteArray :=
-  let b0 := (n      ).toUInt8
-  let b1 := (n >>> 8).toUInt8
-  ByteArray.mk #[b1, b0]
+instance : ToLEByteArray Int8 where
+  toLEByteArray n := toLEByteArray n.toUInt8
 
-def _root_.UInt32.toLEByteArray (n : UInt32) : ByteArray :=
+instance : ToBEByteArray Int8 where
+  toBEByteArray n := toBEByteArray n.toUInt8
+
+instance : ToLEByteArray UInt16 where
+  toLEByteArray n :=
+    let b0 := (n      ).toUInt8
+    let b1 := (n >>> 8).toUInt8
+    ByteArray.mk #[b0, b1]
+
+instance : ToBEByteArray UInt16 where
+  toBEByteArray n :=
+    let b0 := (n      ).toUInt8
+    let b1 := (n >>> 8).toUInt8
+    ByteArray.mk #[b1, b0]
+
+instance : ToLEByteArray Int16 where
+  toLEByteArray n := toLEByteArray n.toUInt16
+
+instance : ToBEByteArray Int16 where
+  toBEByteArray n := toBEByteArray n.toUInt16
+
+instance : ToLEByteArray UInt32 where
+  toLEByteArray n :=
   let b0 := (n       ).toUInt8
   let b1 := (n >>>  8).toUInt8
   let b2 := (n >>> 16).toUInt8
   let b3 := (n >>> 24).toUInt8
   ByteArray.mk #[b0, b1, b2, b3]
 
-def _root_.UInt32.toBEByteArray (n : UInt32) : ByteArray :=
-  let b0 := (n       ).toUInt8
-  let b1 := (n >>>  8).toUInt8
-  let b2 := (n >>> 16).toUInt8
-  let b3 := (n >>> 24).toUInt8
-  ByteArray.mk #[b3, b2, b1, b0]
+instance : ToBEByteArray UInt32 where
+  toBEByteArray n :=
+    let b0 := (n       ).toUInt8
+    let b1 := (n >>>  8).toUInt8
+    let b2 := (n >>> 16).toUInt8
+    let b3 := (n >>> 24).toUInt8
+    ByteArray.mk #[b3, b2, b1, b0]
 
-def _root_.UInt64.toLEByteArray (n : UInt64) : ByteArray :=
-  let b0 := (n       ).toUInt8
-  let b1 := (n >>>  8).toUInt8
-  let b2 := (n >>> 16).toUInt8
-  let b3 := (n >>> 24).toUInt8
-  let b4 := (n >>> 32).toUInt8
-  let b5 := (n >>> 40).toUInt8
-  let b6 := (n >>> 48).toUInt8
-  let b7 := (n >>> 56).toUInt8
-  ByteArray.mk #[b0, b1, b2, b3, b4, b5, b6, b7]
+instance : ToLEByteArray Int32 where
+  toLEByteArray n := toLEByteArray n.toUInt32
 
-def _root_.UInt64.toBEByteArray (n : UInt64) : ByteArray :=
-  let b0 := (n       ).toUInt8
-  let b1 := (n >>>  8).toUInt8
-  let b2 := (n >>> 16).toUInt8
-  let b3 := (n >>> 24).toUInt8
-  let b4 := (n >>> 32).toUInt8
-  let b5 := (n >>> 40).toUInt8
-  let b6 := (n >>> 48).toUInt8
-  let b7 := (n >>> 56).toUInt8
-  ByteArray.mk #[b7, b6, b5, b4, b3, b2, b1, b0]
+instance : ToBEByteArray Int32 where
+  toBEByteArray n := toBEByteArray n.toUInt32
 
-def _root_.Int8.toLEByteArray (n : Int8) : ByteArray := n.toUInt8.toLEByteArray
-def _root_.Int16.toLEByteArray (n : Int16) : ByteArray := n.toUInt16.toLEByteArray
-def _root_.Int32.toLEByteArray (n : Int32) : ByteArray := n.toUInt32.toLEByteArray
-def _root_.Int64.toLEByteArray (n : Int64) : ByteArray := n.toUInt64.toLEByteArray
-def _root_.Int8.toBEByteArray (n : Int8) : ByteArray := n.toUInt8.toBEByteArray
-def _root_.Int16.toBEByteArray (n : Int16) : ByteArray := n.toUInt16.toBEByteArray
-def _root_.Int32.toBEByteArray (n : Int32) : ByteArray := n.toUInt32.toBEByteArray
-def _root_.Int64.toBEByteArray (n : Int64) : ByteArray := n.toUInt64.toBEByteArray
+instance : ToLEByteArray UInt64 where
+  toLEByteArray n :=
+    let b0 := (n       ).toUInt8
+    let b1 := (n >>>  8).toUInt8
+    let b2 := (n >>> 16).toUInt8
+    let b3 := (n >>> 24).toUInt8
+    let b4 := (n >>> 32).toUInt8
+    let b5 := (n >>> 40).toUInt8
+    let b6 := (n >>> 48).toUInt8
+    let b7 := (n >>> 56).toUInt8
+    ByteArray.mk #[b0, b1, b2, b3, b4, b5, b6, b7]
+
+instance : ToBEByteArray UInt64 where
+  toBEByteArray n :=
+    let b0 := (n       ).toUInt8
+    let b1 := (n >>>  8).toUInt8
+    let b2 := (n >>> 16).toUInt8
+    let b3 := (n >>> 24).toUInt8
+    let b4 := (n >>> 32).toUInt8
+    let b5 := (n >>> 40).toUInt8
+    let b6 := (n >>> 48).toUInt8
+    let b7 := (n >>> 56).toUInt8
+    ByteArray.mk #[b7, b6, b5, b4, b3, b2, b1, b0]
+
+instance : ToLEByteArray Int64 where
+  toLEByteArray n := toLEByteArray n.toUInt64
+
+instance : ToBEByteArray Int64 where
+  toBEByteArray n := toBEByteArray n.toUInt64
 
 end TensorLib
